Improvements to hvec

src/hvec.v
@@ -53,6 +53,7 @@ Section ilist.
   Equations ilist_lookup {A} (As : ilist A) (i : fin (ilen As)) : A :=
   | icons x _, 0%fin => x
   | icons _ xs, FS i => ilist_lookup xs i.
+  Global Transparent ilist_lookup.
 
   (* Lookup in a [ilist Type] with [unit] as a fallback. *)
   Fixpoint ilist_type_lookup (As : ilist Type) (i : nat) : Type :=
@@ -65,92 +66,110 @@ Section ilist.
         end
     end.
 
-  Equations ilist_lookup_fin (As : ilist Type) (i : fin (ilen As)) : Type :=
-    | icons t ts, 0%fin := t;
-    | icons t ts, FS i' := ilist_lookup_fin ts i'.
+  Fixpoint iapp {A} (As Bs : ilist A) : ilist A :=
+    match As with inil => Bs | icons A As => icons A (iapp As Bs) end.
+
+  Fixpoint iimpl (As : ilist A) (B : Type) : Type :=
+    match As with inil => B | icons A As => F A → iimpl As B end.
 
 End ilist.
 
+(** A telescope inspired notation for [iimpl]. *)
+Notation "As -h> B" :=
+  (iimpl As B) (at level 99, B at level 200, right associativity).
+
 #[global] Infix "👀" := ilist_lookup (at level 20).
 
-(* We call it [hvec] just to distinguish is from the stdpp's [hlist]. *)
-Inductive hvec : ilist Type → Type :=
-  | hnil : hvec inil
-  | hcons {A As} : A → hvec As → hvec (icons A As).
+(* We call it [hvec] just to distinguish is from the stdpp's [hlist]. We
+parameterize [hvec] by a type [A] and a family [F] over the type. The key
+benefit of this is that we then know that the elements in the elements in [hvec]
+all have the shape [F x] for some [x : A].
+
+For instance, [A] might be [Type] [F] might be [λ x, x * x]. We would then know
+that all elements in the list are pair. Furthermore, Coq is able to compute this
+fact in some circumstantes. In particular [hvec_lookup] we can a priori know the
+shape of the returned type without knowing the specific index and Coq can
+compute with this fact.  *)
+Inductive hvec {A : Type} (F : A → Type) : ilist A → Type :=
+  | hnil : hvec F inil
+  | hcons {x As} : F x → hvec F As → hvec F (icons x As).
+
+Arguments hnil {A F}.
+Arguments hcons {A F} {_ _} a l.
+
+Definition hvec_ty := @hvec Type (λ T, T).
 
 Derive Signature NoConfusion NoConfusionHom for hvec.
 Derive Subterm for hvec.
 
-Fixpoint tapp (As Bs : ilist Type) : ilist Type :=
-  match As with inil => Bs | icons A As => icons A (tapp As Bs) end.
-Fixpoint happ {As Bs} (xs : hvec As) (ys : hvec Bs) : hvec (tapp As Bs) :=
-  match xs with hnil => ys | hcons x xs => hcons x (happ xs ys) end.
+Section hvec.
+  Context {A : Type} {F : A → Type}.
 
-Definition hhead {A As} (xs : hvec (icons A As)) : A :=
-  match xs with hnil => () | hcons x _ => x end.
-Definition htail {A As} (xs : hvec (icons A As)) : hvec As :=
-  match xs with hnil => () | hcons _ xs => xs end.
+  Fixpoint happ {As Bs} (xs : hvec F As) (ys : hvec F Bs) : hvec F (iapp As Bs) :=
+    match xs with hnil => ys | hcons x xs => hcons x (happ xs ys) end.
 
-Fixpoint hheads {As Bs} : hvec (tapp As Bs) → hvec As :=
-  match As with
-  | inil => λ _, hnil
-  | icons _ _ => λ xs, hcons (hhead xs) (hheads (htail xs))
-  end.
-Fixpoint htails {As Bs} : hvec (tapp As Bs) → hvec Bs :=
-  match As with
-  | inil => id
-  | icons _ _ => λ xs, htails (htail xs)
-  end.
+  Definition hhead {A As} (xs : hvec F (icons A As)) : F A :=
+    match xs with hnil => () | hcons x _ => x end.
+  Definition htail {A As} (xs : hvec F (icons A As)) : hvec F As :=
+    match xs with hnil => () | hcons _ xs => xs end.
 
-Fixpoint himpl (As : ilist Type) (B : Type) : Type :=
-  match As with inil => B | icons A As => A → himpl As B end.
+  Fixpoint hheads {As Bs} : hvec F (iapp As Bs) → hvec F As :=
+    match As with
+    | inil => λ _, hnil
+    | icons _ _ => λ xs, hcons (hhead xs) (hheads (htail xs))
+    end.
+  Fixpoint htails {As Bs} : hvec F (iapp As Bs) → hvec F Bs :=
+    match As with
+    | inil => id
+    | icons _ _ => λ xs, htails (htail xs)
+    end.
 
-(** A telescope inspired notation for [himpl]. *)
-Notation "As -h> B" :=
-  (himpl As B) (at level 99, B at level 200, right associativity).
+  Definition hinit {B} (y : B) : himpl inil B := y.
+  Definition hlam {x As B} (f : F x → himpl As B) : himpl (icons x As) B := f.
+  Global Arguments hlam _ _ _ _ _ / : assert.
 
-Definition hinit {B} (y : B) : himpl inil B := y.
-Definition hlam {A As B} (f : A → himpl As B) : himpl (icons A As) B := f.
-Global Arguments hlam _ _ _ _ _ / : assert.
+  Definition huncurry {As B} (f : himpl As B) (xs : hvec F As) : B :=
+    (fix go {As} xs :=
+      match xs in hvec _ As return himpl As B → B with
+      | hnil => λ f, f
+      | hcons x xs => λ f, go xs (f x)
+      end) _ xs f.
+  Coercion huncurry : himpl >-> Funclass.
 
-Definition huncurry {As B} (f : himpl As B) (xs : hvec As) : B :=
-  (fix go {As} xs :=
-    match xs in hvec As return himpl As B → B with
-    | hnil => λ f, f
-    | hcons x xs => λ f, go xs (f x)
-    end) _ xs f.
-Coercion huncurry : himpl >-> Funclass.
+  Fixpoint hcurry {As B} : (hvec F As → B) → himpl As B :=
+    match As with
+    | inil => λ f, f hnil
+    | icons x xs => λ f, hlam (λ x, hcurry (f ∘ hcons x))
+    end.
 
-Fixpoint hcurry {As B} : (hvec As → B) → himpl As B :=
-  match As with
-  | inil => λ f, f hnil
-  | icons x xs => λ f, hlam (λ x, hcurry (f ∘ hcons x))
-  end.
+  Lemma huncurry_curry {As B} (f : hvec F As → B) xs :
+    huncurry (hcurry f) xs = f xs.
+  Proof. by induction xs as [|? As x xs IH]; simpl; rewrite ?IH. Qed.
 
-Lemma huncurry_curry {As B} (f : hvec As → B) xs :
-  huncurry (hcurry f) xs = f xs.
-Proof. by induction xs as [|A As x xs IH]; simpl; rewrite ?IH. Qed.
+  Fixpoint hcompose {As B C} (f : B → C) {struct As} : himpl As B → himpl As C :=
+    match As with
+    | inil => f
+    | icons A As => λ g, hlam (λ x, hcompose f (g x))
+    end.
 
-Fixpoint hcompose {As B C} (f : B → C) {struct As} : himpl As B → himpl As C :=
-  match As with
-  | inil => f
-  | icons A As => λ g, hlam (λ x, hcompose f (g x))
-  end.
+  Compute (icons nat (icons bool (icons Z inil))) 👀 1%fin.
 
-Compute (icons nat (icons bool (icons Z inil))) 👀 1%fin.
+  (* Infix "👀" := ilist_type_lookup (at level 20). *)
+  (* Fixpoint hvec_lookup (As : ilist Type) (l : hvec F As) : *)
+  (*     ∀ (i : nat), ilist_type_lookup As i := *)
+  (*   match l in hvec F As return ∀ i : nat, As 👀 i with *)
+  (*   | hnil => λ i, tt *)
+  (*   | @hcons A As' x xs => λ i : nat, *)
+  (*       match i return ((icons A As') 👀 i) with *)
+  (*       | 0 => x *)
+  (*       | S i' => hvec_lookup As' xs i' *)
+  (*       end *)
+  (*   end. *)
 
-(* Infix "👀" := ilist_type_lookup (at level 20). *)
-(* Fixpoint hvec_lookup (As : ilist Type) (l : hvec As) : *)
-(*     ∀ (i : nat), ilist_type_lookup As i := *)
-(*   match l in hvec As return ∀ i : nat, As 👀 i with *)
-(*   | hnil => λ i, tt *)
-(*   | @hcons A As' x xs => λ i : nat, *)
-(*       match i return ((icons A As') 👀 i) with *)
-(*       | 0 => x *)
-(*       | S i' => hvec_lookup As' xs i' *)
-(*       end *)
-(*   end. *)
+  Equations hvec_lookup {As} (l : hvec F As) (i : fin (ilen As)) : F (As 👀 i) :=
+    hvec_lookup (hcons xx _) 0%fin := xx ;
+    hvec_lookup (hcons _ xs) (FS i') := hvec_lookup xs i'.
 
-Equations ilist_lookup_vec {As} (l : hvec As) (i : fin (ilen As)) : As 👀 i :=
-| hcons x _, 0%fin := x
-| hcons _ xs, FS i' := ilist_lookup_vec xs i'.
+End hvec.
+
+#[global] Infix "👀" := hvec_lookup (at level 20).
